

Abstract—

1 PROBLEM

Find the foot of the perpendicular for a point on the line of intersection of planes $9x^2 - 4y^2 + z^2 - 6xz - 4y - 1 = 0$ on to the plane containing the point $(-1, -4, 3)$.

2 SOLUTION

Given the equation of two intersecting planes is
 $9x^2 - 4y^2 + z^2 - 6xz - 4y - 1 = 0$ (2.0.1)

1) Second order equation in terms of matrices:

The general equation of a second order algebraic surface is given by

$$ax^2 + by^2 + cz^2 + 2dxy + 2exz + 2fyz + 2lx + 2my + 2nz + q = 0. \quad (2.0.2)$$

This equation can be written as:-

$$\mathbf{x}^T \mathbf{V} \mathbf{x} + 2\mathbf{u}^T \mathbf{x} + f = 0 \quad (2.0.3)$$

$$\mathbf{V} = \begin{pmatrix} a & d & e \\ d & b & f \\ e & f & c \end{pmatrix} \quad \mathbf{u} = \begin{pmatrix} l \\ m \\ n \end{pmatrix} \quad (2.0.4)$$

Substituting values from the given equation (2.0.1), we get,

$$\mathbf{x}^T \begin{pmatrix} 9 & 0 & -6 \\ 0 & -4 & 0 \\ -6 & 0 & 1 \end{pmatrix} \mathbf{x} + 2 \begin{pmatrix} 0 \\ -2 \\ 0 \end{pmatrix}^T \mathbf{x} - 1 = 0 \quad (2.0.5)$$

$$\mathbf{V} = \begin{pmatrix} 9 & 0 & -6 \\ 0 & -4 & 0 \\ -6 & 0 & 1 \end{pmatrix} \quad \mathbf{u} = \begin{pmatrix} 0 \\ -2 \\ 0 \end{pmatrix} \quad f = -1 \quad (2.0.6)$$

a) The eigen values of matrix \mathbf{V} can be calculated as:-

$$|\mathbf{V} - \lambda \mathbf{I}| = 0 \quad (2.0.7)$$

$$\begin{vmatrix} 9 - \lambda & 0 & -6 \\ 0 & -4 - \lambda & 0 \\ -6 & 0 & 1 - \lambda \end{vmatrix} = 0 \quad (2.0.8)$$

$$\Rightarrow -\lambda^3 + 6\lambda^2 + 67\lambda + 108 = 0 \quad (2.0.9)$$

$$(-\lambda - 4)(\lambda^2 - 10\lambda - 27) = 0 \quad (2.0.10)$$

From above, we get,

$$\lambda_1 = -4 \quad (2.0.11)$$

$$\lambda_2 = -2\sqrt{13} + 5 \quad (2.0.12)$$

$$\lambda_3 = 2\sqrt{13} + 5 \quad (2.0.13)$$

The corresponding eigen vectors for these eigen values are:-

$$\text{for } \lambda_1 = -4, \mathbf{v}_1 = \begin{pmatrix} 0 \\ 1 \\ 0 \end{pmatrix} \quad (2.0.14)$$

$$\text{for } \lambda_2 = -2\sqrt{13} + 5, \mathbf{v}_2 = \begin{pmatrix} \frac{\sqrt{13}-2}{3} \\ 0 \\ 1 \end{pmatrix} \quad (2.0.15)$$

$$\text{for } \lambda_3 = 2\sqrt{13} + 5, \mathbf{v}_3 = \begin{pmatrix} \frac{-\sqrt{13}-2}{3} \\ 0 \\ 1 \end{pmatrix} \quad (2.0.16)$$

Eigen vectors matrix is

$$\begin{pmatrix} 0 & \frac{\sqrt{13}-2}{3} & \frac{-\sqrt{13}-2}{3} \\ 1 & 0 & 0 \\ 0 & 1 & 1 \end{pmatrix} \quad (2.0.17)$$

The normalizing these values, we obtain

$$\begin{pmatrix} 0 & \frac{\sqrt{13}-2}{\sqrt{26-4\sqrt{13}}} & \frac{-\sqrt{13}-2}{\sqrt{26+4\sqrt{13}}} \\ 1 & 0 & 0 \\ 0 & \frac{3}{\sqrt{26-4\sqrt{13}}} & \frac{3}{\sqrt{26+4\sqrt{13}}} \end{pmatrix} \quad (2.0.18)$$

b) Affine transformation:

We can obtain the affine transformation for equation at (2.0.3) by taking the value of \mathbf{x} as:

$$\mathbf{x} = \mathbf{P}\mathbf{y} + \mathbf{c} \quad (2.0.19)$$

such that

$$\mathbf{P}^T \mathbf{V} \mathbf{P} = \mathbf{D} \quad (2.0.20)$$

$$\mathbf{D} = \begin{pmatrix} \lambda_1 & 0 & 0 \\ 0 & \lambda_2 & 0 \\ 0 & 0 & \lambda_3 \end{pmatrix} \quad (2.0.21)$$

and \mathbf{P} is the transformation matrix and can be given by the normalized eigen vectors of matrix \mathbf{V} . Therefore,

$$\mathbf{P} = \begin{pmatrix} 0 & \frac{\sqrt{13}-2}{\sqrt{26-4\sqrt{13}}} & \frac{-\sqrt{13}-2}{\sqrt{26+4\sqrt{13}}} \\ 1 & 0 & 0 \\ 0 & \frac{3}{\sqrt{26-4\sqrt{13}}} & \frac{3}{\sqrt{26+4\sqrt{13}}} \end{pmatrix} \quad (2.0.22)$$

Also, $\mathbf{P}^T = \mathbf{P}^{-1}$

$$\begin{aligned} \mathbf{P}^T \mathbf{V} \mathbf{P} &= \begin{pmatrix} 0 & 1 & 0 \\ \frac{\sqrt{13}-2}{\sqrt{26-4\sqrt{13}}} & 0 & \frac{3}{\sqrt{26-4\sqrt{13}}} \\ \frac{-\sqrt{13}-2}{\sqrt{26+4\sqrt{13}}} & 0 & \frac{3}{\sqrt{26+4\sqrt{13}}} \end{pmatrix} \\ &\begin{pmatrix} 9 & 0 & -6 \\ 0 & -4 & 0 \\ -6 & 0 & 1 \end{pmatrix} \begin{pmatrix} 0 & \frac{\sqrt{13}-2}{\sqrt{26-4\sqrt{13}}} & \frac{-\sqrt{13}-2}{\sqrt{26+4\sqrt{13}}} \\ 1 & 0 & 0 \\ 0 & \frac{3}{\sqrt{26-4\sqrt{13}}} & \frac{3}{\sqrt{26+4\sqrt{13}}} \end{pmatrix} \\ &\quad (2.0.23) \end{aligned}$$

$$= \begin{pmatrix} -4 & 0 & 0 \\ 0 & -2\sqrt{13}+5 & 0 \\ 0 & 0 & 2\sqrt{13}+5 \end{pmatrix} = \mathbf{D} \quad (2.0.24)$$

(2.0.3) can be expressed as:

$$\mathbf{y}^T \mathbf{D} \mathbf{y} = \mathbf{u}^T \mathbf{V}^{-1} \mathbf{u} - f \quad \therefore |\mathbf{V}| \neq 0 \quad (2.0.25)$$

$$\begin{aligned} &\mathbf{u}^T \mathbf{V}^{-1} \mathbf{u} \\ &= (0 \quad -2 \quad 0) \begin{pmatrix} \frac{-1}{27} & 0 & \frac{-2}{9} \\ 0 & \frac{-1}{4} & 0 \\ \frac{-2}{9} & 0 & \frac{-1}{3} \end{pmatrix} \begin{pmatrix} 0 \\ -2 \\ 0 \end{pmatrix} \\ &\quad = -1 \quad (2.0.26) \end{aligned}$$

Therefore, we obtain

$$\mathbf{y}^T \begin{pmatrix} -4 & 0 & 0 \\ 0 & -2\sqrt{13}+5 & 0 \\ 0 & 0 & 2\sqrt{13}+5 \end{pmatrix} \mathbf{y} = 0 \quad (2.0.27)$$

Expressing in terms of individual plane equations, we get

$$(3x - 2y - z - 1)(3x + 2y - z + 1) = 0 \quad (2.0.28)$$